Metalean/TypeTheory/NaturalModel/Morphism.lean
@@ -5,7 +5,8 @@ Authors: Jeremy Chen
 -/
 module
 
-public import Metalean.TypeTheory.NaturalModel.Extension
+public import Metalean.TypeTheory.NaturalModel.Pi
+public import Metalean.TypeTheory.NaturalModel.Sort
 
 @[expose] public noncomputable section
 
@@ -37,5 +38,39 @@ structure Morphism where
     IsIso (substTerm (onTy Γ A) (onCtx.map (disp A))
       (onTm _ (genericTerm A)) (by
         rw [onTm_typing, ← onTy_subst, genericTerm_typing, Equiv.symm_apply_apply]))
+
+namespace Morphism
+
+variable {Ty Ty'} (F : Morphism Ty Ty') {Γ : C}
+
+def extComparison (A : y Γ ⟶ Ty) : F.onCtx.obj (ext A) ⟶ ext (F.onTy Γ A) :=
+  substTerm (F.onTy Γ A) (F.onCtx.map (disp A)) (F.onTm _ (genericTerm A)) (by
+    rw [F.onTm_typing, ← F.onTy_subst, genericTerm_typing, Equiv.symm_apply_apply])
+
+instance isIso_extComparison (A : y Γ ⟶ Ty) : IsIso (F.extComparison A) :=
+  F.preservesExt A
+
+def extIso (A : y Γ ⟶ Ty) : F.onCtx.obj (ext A) ≅ ext (F.onTy Γ A) :=
+  asIso (F.extComparison A)
+
+variable {ℓ : Nat} [HasSorts Ty Tm ℓ] [HasSorts Ty' Tm' ℓ]
+
+class PreservesSorts : Prop where
+  onTy_sort {Γ : C} (v : Level ℓ) :
+    F.onTy Γ (HasSorts.sort v Γ) = HasSorts.sort v (F.onCtx.obj Γ)
+  onTy_el {Γ : C} (v : Level ℓ) (t : Tm.obj (op Γ))
+    (ht : ℳ.typing.app (op Γ) t = yonedaEquiv (HasSorts.sort v Γ)) :
+    F.onTy Γ (HasSorts.el v t ht) =
+      HasSorts.el v (F.onTm Γ t) (by
+        rw [F.onTm_typing, ht, Equiv.symm_apply_apply, onTy_sort])
+
+variable [HasPi Ty Tm] [HasPi Ty' Tm']
+
+class PreservesPi : Prop where
+  onTy_piCode {Γ : C} (A : y Γ ⟶ Ty) (B : y (ext A) ⟶ Ty) :
+    F.onTy Γ (piCode A B) =
+      piCode (F.onTy Γ A) (y (inv (F.extComparison A)) ≫ F.onTy (ext A) B)
+
+end Morphism
 
 end Metalean.TypeTheory.NaturalModel
